WIP

compose/ModTuple.v
@@ -10,8 +10,10 @@ Require Import Integers.
 Require Import ASTC.
 Require Import Maps.
 Require Import AxiomsC.
-Require Import LinkingC.
+Require Import LinkingC LinkingProps SemProps ModSemProps.
+Require Import BehaviorsC.
 
+Require Import Simulation.
 Require Import Mod Sem ModSem.
 Require Import Any.
 Require Import Program.
@@ -300,6 +302,8 @@ To do this, I will require initial_state to be deterministic.
 
 End MODSEMTUPLE.
 
+Arguments StackNil {msdl} {msdr}.
+
 
 (*** if we put "MODTUPLE" section inside "ModTuple" module, "Print ModTuple" will be very messy ***)
 Module ModSemTuple.
@@ -347,6 +351,199 @@ End MODTUPLE.
 
 Module ModTuple.
   Definition t := Eval red in t'.
+
+  Section PROPS.
+    Variable mdl mdr: Mod.t.
+    Variable sk: Sk.t.
+    Variable midx: string.
+    Variable ctx1 ctx2: list Mod.t.
+    Hypothesis (LINKSK: link (mdl: Sk.t) mdr = Some sk).
+    Hypothesis (MIDXL: mdl.(Mod.midx) = Some midx).
+    Hypothesis (WFL: Sk.wf mdl).
+    Hypothesis (WFR: Sk.wf mdr).
+
+    Let WFLINK: Sk.wf (t mdl mdr sk midx).
+    Proof.
+      eapply link_preserves_wf_sk in LINKSK; et.
+    Qed.
+
+    Let LINKSAME: forall
+        (* (WFL: Sk.wf mdl) *)
+        (* (WFR: Sk.wf mdr) *)
+        (* (WF: Sk.wf sk) *)
+        (* (WFCTX1: forall md (IN: In md ctx1), Sk.wf md) *)
+        (* (WFCTX2: forall md (IN: In md ctx2), Sk.wf md) *)
+        (WF: forall md (IN: In md (ctx1 ++ mdl :: mdr :: ctx2)), Sk.wf md)
+      ,
+        <<EQ: link_sk (ctx1 ++ [mdl] ++ [mdr] ++ ctx2) = link_sk (ctx1 ++ [(t mdl mdr sk midx)] ++ ctx2)>>.
+    Proof.
+      i. erewrite link_sk_prepend_eq; eauto.
+      { ss. }
+      unfold t. unfold link_sk. ss.
+      replace (Mod.sk mdl :: Mod.sk mdr :: map Mod.sk ctx2)
+        with ([Mod.sk mdl ; Mod.sk mdr] ++ map Mod.sk ctx2) by ss.
+      erewrite link_list_assoc_one; ss; try eapply WF; ss; try rewrite in_app; ss; eauto.
+      ii. rewrite in_map_iff in *. des; clarify; et.
+      try eapply WF; ss; try rewrite in_app; ss; eauto.
+    Qed.
+
+    Section MATCH.
+      Variable skenv_link: SkEnv.t.
+      Let msdl: ModSem.t := (Mod.get_modsem mdl skenv_link mdl.(Mod.data)).
+      Let msdr: ModSem.t := (Mod.get_modsem mdr skenv_link mdr.(Mod.data)).
+      Let ms_link: ModSem.t := (ModSemTuple.t (Mod.get_modsem mdl skenv_link mdl.(Mod.data))
+                                              (Mod.get_modsem mdr skenv_link mdr.(Mod.data)) sk skenv_link midx).
+
+      Inductive match_focus_stack: (stack msdl msdr) -> list Frame.t -> Prop :=
+      | match_focus_stack_nil
+        :
+          match_focus_stack StackNil nil
+      | match_focus_stack_cons_dl
+          stl0 stk frs
+          (TL: match_focus_stack stk frs)
+        :
+          match_focus_stack (StackCons dl stl0 stk) ((Frame.mk msdl stl0) :: frs)
+      | match_focus_stack_cons_dr
+          stl0 stk frs
+          (TL: match_focus_stack stk frs)
+        :
+          match_focus_stack (StackCons dr stl0 stk) ((Frame.mk msdr stl0) :: frs)
+      .
+
+      (***
+          Q: state maintains "owned_heap"... if it is outdated, what is the meaning of it?
+          A(?): it is nothing special -- it is almost the same with "memory" (which is hidden inside state too)
+          No(!): owned_heap is in (1) msl/msr.state (hidden), (2) ModSemTuple.state, and (3) Sem.state
+       ***)
+
+      (***
+          Note: src synchronizes (update global Ohs) less than target.
+          WTS: (at least) when synchronization happens, it should coincide
+       ***)
+
+      (*** ohs_tgt is the latest known global Ohs. src's internal Ohs should be consistent with it ***)
+      Inductive match_stacks (ohs_tgt: Ohs): list Frame.t -> list Frame.t -> Prop :=
+      | match_stacks_nil
+        :
+          match_stacks ohs_tgt [] []
+      | match_stacks_cons_ctx
+          tail_src tail_tgt
+          (TAIL: match_stacks ohs_tgt tail_src tail_tgt) hd :
+          match_stacks ohs_tgt (hd :: tail_src) (hd :: tail_tgt)
+      | match_stacks_focus
+          tail_src tail_tgt
+          (TAIL: match_stacks ohs_tgt tail_src tail_tgt)
+          hd_src stk_src oh_src hds_tgt
+          (NNIL: stk_src <> StackNil)
+          (HD: match_focus_stack stk_src hds_tgt)
+          (STK: hd_src = Frame.mk ms_link (stk_src, oh_src))
+          (OHL: ohs_tgt msdl.(ModSem.midx) = upcast (fst oh_src))
+          (OHR: ohs_tgt msdr.(ModSem.midx) = upcast (snd oh_src))
+        :
+          match_stacks ohs_tgt (hd_src :: tail_src) (hds_tgt ++ tail_tgt)
+      .
+
+      Lemma match_stacks_right_nil
+            ohs_tgt frs
+            (STK: match_stacks ohs_tgt frs []) :
+        <<NIL: frs = []>>.
+      Proof.
+        inv STK; ss. destruct hds_tgt, tail_tgt; ss.
+        inv HD; ss.
+      Qed.
+
+      Inductive match_states : Sem.state -> Sem.state -> Prop :=
+      | match_states_normal
+          frs_src frs_tgt ohs_src ohs_tgt
+          (STK: match_stacks ohs_tgt frs_src frs_tgt)
+          (OHS: forall mj (NL: mj <> msdl.(ModSem.midx)) (NR: mj <> msdr.(ModSem.midx)),
+              ohs_src mj = ohs_tgt mj)
+        :
+          match_states (State frs_src ohs_src) (State frs_tgt ohs_tgt)
+      | match_states_call
+          frs_src frs_tgt args ohs_src ohs_tgt
+          (STK: match_stacks ohs_tgt frs_src frs_tgt)
+          (OHS: forall mj (NL: mj <> msdl.(ModSem.midx)) (NR: mj <> msdr.(ModSem.midx)),
+              ohs_src mj = ohs_tgt mj)
+          ohl ohr
+          (OHLR: @downcast ms_link.(ModSem.owned_heap) (ohs_src msdl.(ModSem.midx)) = Some (ohl, ohr))
+          (OHL: @downcast msdl.(ModSem.owned_heap) (ohs_tgt msdl.(ModSem.midx)) = Some ohl)
+          (OHR: @downcast msdr.(ModSem.owned_heap) (ohs_tgt msdr.(ModSem.midx)) = Some ohr)
+        :
+          match_states (Callstate args frs_src ohs_src) (Callstate args frs_tgt ohs_tgt)
+      .
+
+    End MATCH.
+
+    Lemma match_states_xsim
+          skenv_link st_src0 st_tgt0
+          (MATCH: match_states skenv_link st_src0 st_tgt0) :
+      <<XSIM: xsim (sem (ctx1 ++ [mdl] ++ [mdr] ++ ctx2)) (sem (ctx1 ++ [(t mdl mdr sk midx)] ++ ctx2))
+                   bot2 top1 top1 tt st_src0 st_tgt0>>
+    .
+    Proof.
+      revert_until LINKSAME.
+      pcofix CIH. i. pfold.
+      inv MATCH.
+      - (* normal *)
+        ss. destruct frs_src; ss.
+        { inv STK. left. right.
+          econs 1; eauto.
+          econs 1; eauto.
+          - econs 1; eauto. i. inv STEPSRC.
+          - i. ss. inv FINALSRC; ss. }
+        rename t into fr_src.
+        destruct frs_tgt; ss.
+        { exploit match_stacks_right_nil; et. i; des. clarify. }
+        rename t into fr_tgt.
+        ii. clear SSSRC. ss. rewrite LINKTGT in *.
+        destruct (classic (fr_tgt.(Frame.ms).(ModSem.is_call) fr_tgt.(Frame.st))).
+        (* tgt call *)
+        (* fsim *)
+        { left. right. econs; et. econs; et; cycle 1.
+
+        inv STK; ss.
+        + destruct (classic (fr_tgt.(Frame.ms).(ModSem.is_call) fr_tgt.(Frame.st))).
+        
+        ii.
+        admit "".
+      - (* call *)
+        admit "".
+    Qed.
+
+    Theorem merge:
+      <<BEH: improves (sem (ctx1 ++ [mdl] ++ [mdr] ++ ctx2)) (sem (ctx1 ++ [(t mdl mdr sk midx)] ++ ctx2))>>
+    .
+    Proof.
+      eapply bsim_improves; eauto. ss.
+      eapply Simulation.mixed_to_backward_simulation; et.
+      econs. instantiate (1:= bot2). instantiate (1:= unit).
+      econs; ss; try apply preservation_top; et; cycle 1.
+      { ii. des. inv SAFESRC. rewrite <- LINKSAME; et. }
+      econs 1; ss.
+      ii. inv INITSRC; ss. des_ifs.
+      esplits; et.
+      { econs; cycle 1.
+        { eapply initial_state_determ; et. }
+        ss. rewrite <- LINKSAME; et.
+        econs; ss; et.
+        - rewrite <- LINKSAME; et.
+        - i. rewrite in_app_iff in *. ss; des; clarify; try (by eapply WF; ss; try rewrite in_app; ss; et).
+        - admit "ez - nodup".
+      }
+      eapply match_states_xsim with (skenv_link := Sk.load_skenv sk_link); et.
+      econs 2; et.
+      - econs; et.
+      - ii. ss.
+        admit "ez - load_owned_heaps".
+      - admit "ez - load_owned_heaps".
+      - admit "ez - load_owned_heaps".
+      - admit "ez - load_owned_heaps".
+    Unshelve.
+      all: try eapply ModSem.initial_owned_heap.
+    Qed.
+  End PROPS.
+
 End ModTuple.
 Print ModTuple.t.
 
