proof/LinkingProps.v
@@ -1,0 +1,965 @@
+Require Import CoqlibC Maps Postorder.
+Require Import AST Linking.
+Require Import ValuesC Memory GlobalenvsC Events Smallstep.
+Require Import Op Registers ClightC Renumber.
+Require Import CtypesC CtypingC.
+Require Import sflib.
+Require Import IntegersC.
+
+Require Import Simulation.
+Require Import Skeleton Mod ModSem SimMod SimModSem SimSymb SimMem AsmregsC MatchSimModSem.
+(* Require SimMemInjC. *)
+Require SimMemId.
+Require SoundTop.
+Require Import Clightdefs.
+Require Import CtypesC.
+Require Import BehaviorsC.
+Require Import LinkingC2.
+Require Import Simulation Sem SemProps LinkingC.
+
+Set Implicit Arguments.
+
+
+(*** TODO: move to CoqlibC ***)
+Tactic Notation "renames" ident(a) "into"
+       ident(x) :=
+  rename a into x.
+
+Tactic Notation "renames" ident(a) ident(b) "into"
+       ident(x) ident(y) :=
+  rename a into x; rename b into y.
+
+Tactic Notation "renames" ident(a) ident(b) ident(c) "into"
+       ident(x) ident(y) ident(z) :=
+  rename a into x; rename b into y; rename c into z.
+
+Tactic Notation "renames" ident(a) ident(b) ident(c) ident(d) "into"
+       ident(x) ident(y) ident(z) ident(w) :=
+  rename a into x; rename b into y; rename c into z; rename d into w.
+
+
+
+
+Ltac des_bool :=
+  repeat
+    (match goal with
+     | H: andb ?a ?b = true |- _ =>
+       apply andb_true_iff in H;
+       let H1 := fresh H in
+       let H2 := fresh H in
+       destruct H as [H1 H2]
+     | H: andb ?a ?b = false |- _ => apply andb_false_iff in H
+     end).
+
+Ltac des_matchH H n :=
+  match goal with
+  | H':context [ if ?X then _ else _ ] |- _ =>
+    let n' := fresh n in
+    check_equal H' H; destruct X eqn: n
+  | H':context [ match ?X with _ => _ end ] |- _ =>
+    let n' := fresh n in
+    check_equal H' H; destruct X eqn: n
+  end.
+
+Definition link_assoc F `{Linker F} : Prop :=
+  forall (f0 f1 f2: F),
+    match (link f0 f1) with
+    | Some f01 => link f01 f2
+    | _ => None
+    end =
+    match (link f1 f2) with
+    | Some f12 => link f0 f12
+    | _ => None
+    end.
+Arguments link_assoc F {_}.
+
+Require Import mktac.
+
+Lemma classify_init_case l
+  :
+    (<<EXTERN: l = []>>) \/
+    (<<COMMON: exists sz, l = [Init_space sz]>>) \/
+    (<<DEFINITIVE: classify_init l = Init_definitive l>>).
+Proof.
+  destruct l; ss; eauto. right. destruct i, l; ss; eauto.
+Qed.
+
+Lemma Z_max_double n m
+  :
+    Z.max (Z.max n m) m = Z.max n m.
+Proof.
+  unfold Z.max in *. des_ifs; clarify.
+  - eapply Z.compare_eq in Heq0. eauto.
+  - congruence.
+Qed.
+
+Lemma init_data_list_size_max_zero l
+  :
+    Z.max (init_data_list_size l) 0 = (init_data_list_size l).
+Proof.
+  unfold Z.max. des_ifs.
+  set (init_data_list_size_pos l).
+  exfalso. unfold Z.ge in *. auto.
+Qed.
+
+Lemma link_varinit_assoc
+  :
+    link_assoc (list init_data).
+Proof.
+  ii. Local Transparent Linker_varinit. ss. unfold link_varinit.
+  set (classify_init_case f0).
+  set (classify_init_case f1).
+  set (classify_init_case f2). des; clarify; ss; des_ifs; ss; clarify; zsimpl.
+  - rewrite Z_max_double in *. clarify.
+  - repeat rewrite init_data_list_size_max_zero in *. f_equal. auto.
+  - rewrite Z_max_double in *. clarify.
+  - rewrite Z_max_double in *. clarify.
+  - repeat rewrite init_data_list_size_max_zero in *. f_equal. auto.
+  - repeat rewrite init_data_list_size_max_zero in *. clarify.
+  - repeat rewrite init_data_list_size_max_zero in *. clarify.
+  - repeat rewrite init_data_list_size_max_zero in *. f_equal. auto.
+  - repeat rewrite init_data_list_size_max_zero in *. clarify.
+  - repeat rewrite init_data_list_size_max_zero in *. clarify.
+Qed.
+
+Lemma link_vardef_assoc
+      V `{Linker V}
+      (ASSOCV: link_assoc V)
+  :
+    link_assoc (globvar V).
+Proof.
+  ii. Local Transparent Linker_vardef. ss. unfold link_vardef. des_ifs; ss.
+  - f_equal. f_equal; ss.
+    + specialize (ASSOCV (gvar_info f0) (gvar_info f1) (gvar_info f2)).
+      rewrite Heq3 in *. rewrite Heq7 in *. rewrite Heq0 in *. rewrite Heq4 in *. clarify.
+    + specialize (link_varinit_assoc (gvar_init f0) (gvar_init f1) (gvar_init f2)). i. ss.
+      rewrite Heq10 in *. rewrite Heq8 in *. rewrite Heq1 in *. rewrite Heq5 in *. clarify.
+  - exfalso. unfold proj_sumbool, andb in *. des_ifs.
+  - exfalso.
+    specialize (link_varinit_assoc (gvar_init f0) (gvar_init f1) (gvar_init f2)). i. ss.
+    rewrite Heq9 in *. rewrite Heq7 in *. rewrite Heq1 in *. rewrite Heq5 in *. clarify.
+  - exfalso.
+    specialize (ASSOCV (gvar_info f0) (gvar_info f1) (gvar_info f2)).
+    rewrite Heq3 in *. rewrite Heq5 in *. rewrite Heq0 in *. rewrite Heq4 in *. clarify.
+  - exfalso. destruct f0, f1, f2. ss. unfold andb, eqb in *. des_ifs.
+  - exfalso.
+    specialize (link_varinit_assoc (gvar_init f0) (gvar_init f1) (gvar_init f2)). i. ss.
+    rewrite Heq7 in *. rewrite Heq5 in *. rewrite Heq1 in *. clarify.
+  - exfalso.
+    specialize (ASSOCV (gvar_info f0) (gvar_info f1) (gvar_info f2)).
+    rewrite Heq5 in *. rewrite Heq4 in *. rewrite Heq0 in *. clarify.
+  - exfalso. destruct f0, f1, f2. ss. unfold andb, eqb in *. des_ifs.
+  - exfalso.
+    specialize (link_varinit_assoc (gvar_init f0) (gvar_init f1) (gvar_init f2)). i. ss.
+    rewrite Heq9 in *. rewrite Heq7 in *. rewrite Heq4 in *. rewrite Heq1 in *. clarify.
+  - exfalso.
+    specialize (ASSOCV (gvar_info f0) (gvar_info f1) (gvar_info f2)).
+    rewrite Heq1 in *. rewrite Heq5 in *. rewrite Heq2 in *. rewrite Heq0 in *. clarify.
+  - exfalso. unfold proj_sumbool, andb in *. des_ifs.
+  - exfalso.
+    specialize (link_varinit_assoc (gvar_init f0) (gvar_init f1) (gvar_init f2)). i. ss.
+    rewrite Heq7 in *. rewrite Heq5 in *. rewrite Heq2 in *. clarify.
+  - exfalso.
+    specialize (ASSOCV (gvar_info f0) (gvar_info f1) (gvar_info f2)).
+    rewrite Heq0 in *. rewrite Heq4 in *. rewrite Heq1 in *. clarify.
+Qed.
+
+Lemma link_def_assoc
+      F V `{Linker F} `{Linker V}
+      (ASSOCF: link_assoc F)
+      (ASSOCV: link_assoc V)
+  :
+    link_assoc (globdef F V).
+Proof.
+  ii. Local Transparent Linker_def. ss. unfold link_def. des_ifs; repeat f_equal.
+  - specialize (ASSOCF f4 f6 f3).
+    rewrite Heq1 in *. rewrite Heq3 in *. rewrite ASSOCF in *. clarify.
+  - specialize (ASSOCF f4 f5 f3).
+    rewrite Heq1 in *. rewrite Heq3 in *. rewrite ASSOCF in *. clarify.
+  - specialize (ASSOCF f1 f4 f3).
+    rewrite Heq3 in *. rewrite Heq2 in *. rewrite ASSOCF in *. clarify.
+  - specialize (ASSOCF f2 f5 f3).
+    rewrite Heq1 in *. rewrite Heq3 in *. rewrite ASSOCF in *. clarify.
+  - specialize (link_vardef_assoc ASSOCV v1 v3 v0). i. ss.
+    rewrite Heq1 in *. rewrite Heq0 in *. rewrite Heq3 in *. rewrite Heq2 in *. clarify.
+  - specialize (link_vardef_assoc ASSOCV v1 v3 v0). i. ss.
+    rewrite Heq1 in *. rewrite Heq0 in *. rewrite Heq3 in *. rewrite Heq2 in *. clarify.
+  - specialize (link_vardef_assoc ASSOCV v2 v1 v0). i. ss.
+    rewrite Heq3 in *. rewrite Heq0 in *. rewrite Heq2 in *. clarify.
+  - specialize (link_vardef_assoc ASSOCV v1 v3 v0). i. ss.
+    rewrite Heq1 in *. rewrite Heq0 in *. rewrite Heq3 in *. rewrite Heq2 in *. clarify.
+  - specialize (ASSOCF f f4 f1).
+    rewrite Heq2 in *. rewrite Heq1 in *. rewrite Heq0 in *. clarify.
+  - specialize (link_vardef_assoc ASSOCV v v1 v2). i. ss.
+    rewrite Heq2 in *. rewrite Heq1 in *. rewrite Heq0 in *. clarify.
+Qed.
+
+(* above by Minki *)
+
+Lemma link_ef_either
+      e1 e2 f3
+      (L: link (AST.External e1) (AST.External e2) = Some f3)
+  : f3 = AST.External e1 \/ f3 = AST.External e2.
+Proof.
+  unfold link in *. ss.
+  destruct e1, e2; desf; eauto.
+Qed.
+
+(* Lemma link_ef_inv *)
+(*       e1 e2 f3 *)
+(*       (EF1: is_external_ef e1 = true) *)
+(*       (EF2: is_external_ef e2 = true) *)
+(*       (L: link (AST.External e1) (AST.External e2) = Some f3) *)
+(*   : exists e3, f3 = AST.External e3 /\ is_external_ef e3. *)
+(* Proof. *)
+(*   destruct e1; ss. *)
+(*   destruct e2; ss. *)
+(*   desf. eexists. split; eauto. *)
+(* Qed. *)
+
+Lemma link_nef_inv
+      e1 e2 f3
+      (EF1: is_external_ef e1 = false)
+      (EF2: is_external_ef e2 = false)
+      (L: link (AST.External e1) (AST.External e2) = Some f3)
+  : e1 = e2 /\ f3 = AST.External e1.
+Proof.
+  destruct e1; destruct e2; ss; desf.
+Qed.
+
+Lemma link_ef_no
+      e1 e2
+      (EF1: xorb (is_external_ef e1) (is_external_ef e2))
+  : link (AST.External e1) (AST.External e2) = None.
+Proof.
+  destruct e1; destruct e2; desf.
+Qed.
+
+Lemma link_external_assoc e0 e1 e2
+  : match link (AST.External e0) (AST.External e1) with
+    | Some e01 => link e01 (AST.External e2)
+    | None => None
+    end = match link (AST.External e1) (AST.External e2) with
+          | Some e12 => link (AST.External e0) e12
+          | None => None
+          end.
+Proof.
+  destruct (is_external_ef e0) eqn: EXT_EF0;
+    destruct (is_external_ef e1) eqn: EXT_EF1.
+  - destruct e0; ss. destruct e1; ss.
+    destruct (is_external_ef e2) eqn: EXT_EF2.
+    + destruct e2; ss.
+      desf; ss; desf.
+    + exploit (link_ef_no (EF_external name sg) e2); eauto; [desf| ]. i.
+      desf.
+  - exploit (link_ef_no e0 e1); eauto; [desf| ]. i.
+    desf. symmetry.
+    destruct (is_external_ef e2) eqn: EXT_EF2.
+    + exploit (link_ef_no e1 e2); eauto; [desf| ]. i.
+      congruence.
+    + exploit (link_nef_inv e1 e2); eauto. i. des. clarify.
+  - exploit (link_ef_no e0 e1); eauto; [desf| ]. i.
+    desf. symmetry.
+    destruct (is_external_ef e2) eqn: EXT_EF2.
+    + exploit link_ef_either; eauto. i. des; clarify.
+      apply link_ef_no. desf.
+    + exploit (link_ef_no e1 e2); eauto; [desf| ]. i.
+      congruence.
+  - destruct (link (AST.External e0) (AST.External e1)) eqn:L01.
+    + exploit (link_nef_inv e0 e1); eauto. i. des. clarify.
+      destruct (is_external_ef e2) eqn: EXT_EF2.
+      { exploit (link_ef_no e1 e2); eauto; [by desf|]. i.
+        desf. }
+      { desf.
+        exploit (link_nef_inv e1 e2); eauto. i. des. clarify. }
+    + destruct (is_external_ef e2) eqn: EXT_EF2.
+      { exploit (link_ef_no e1 e2); eauto; [by desf|]. i.
+        desf. }
+      { desf.
+        exploit (link_nef_inv e1 e2); eauto. i. des. clarify. }
+Qed.
+
+Lemma link_skfundef_assoc
+  : link_assoc (AST.fundef signature).
+Proof.
+  unfold link_assoc. i.
+  destruct f0 as [s0| e0]; destruct f1 as [s1| e1];
+    destruct f2 as [s2| e2];
+    first [by apply link_external_assoc | ss; desf; ss; desf].
+Qed.
+
+Corollary link_skdef_assoc
+  : link_assoc (AST.globdef (AST.fundef signature) unit).
+Proof.
+  apply link_def_assoc; ss.
+  apply link_skfundef_assoc.
+Qed.
+
+Lemma link_sk_assoc
+      (m1 m2 m3: Sk.t)
+      (WF1: Sk.wf m1)
+      (WF2: Sk.wf m2)
+      (WF3: Sk.wf m3)
+  : match (link m1 m2) with
+    | Some m12 => link m12 m3
+    | _ => None
+    end =
+    match (link m2 m3) with
+    | Some m23 => link m1 m23
+    | _ => None
+    end.
+Proof.
+  Local Transparent Linker_prog Linker_def.
+  destruct (link m2 m3) as [m23|] eqn: L2_3.
+  2: {
+    ss. unfold link_prog in *. desf. ss.
+    exfalso.
+
+    renames Heq Heq1 Heq0 into P2_3F P1_2S P12_3S.
+
+    des_bool. des.
+    { unfold ident_eq in *.
+      unfold proj_sumbool in *. desf.
+      congruence.
+    }
+    renames P1_2S1 P12_3S1 into P1_2S P12_3S.
+
+    rewrite PTree_Properties.for_all_false in P2_3F.
+    destruct P2_3F as [x [d2 [DEF2 L2_3F]]].
+
+    rewrite PTree_Properties.for_all_correct in P1_2S. specialize (P1_2S x).
+    rewrite PTree_Properties.for_all_correct in P12_3S. specialize (P12_3S x).
+
+    destruct ((prog_defmap m1) ! x) as [d1|] eqn: DEF1.
+    - exploit P1_2S; eauto. intro C1_2S. clear P1_2S.
+      unfold link_prog_check in C1_2S.
+      rewrite DEF2 in C1_2S. desf.
+      2: { des_bool. ss. }
+      renames g Heq into d12 L1_2S.
+
+      exploit P12_3S.
+      { rewrite prog_defmap_elements.
+        rewrite PTree.gcombine by ss.
+        rewrite DEF1. rewrite DEF2. ss. eauto.
+      }
+      (* clear - LINK12 C2_3F. intro C12_3. *)
+      clear P12_3S. intro C12_3S.
+      unfold link_prog_check in *.
+      destruct ((prog_defmap m3) ! x) as [d3|] eqn: DEF3; ss.
+
+      des_bool.
+      destruct L2_3F as [? | L2_3F'].
+      { desf. }
+      destruct (link_def d2 d3) as [d23| ] eqn: L2_3F; desf.
+      renames g Heq into d123 L12_3S.
+
+      assert (match link d1 d2 with
+              | Some d12 => link d12 d3
+              | None => None
+              end = match link d2 d3 with
+                    | Some d23 => link d1 d23
+                    | None => None
+                    end).
+      { apply link_def_assoc.
+        - apply link_skfundef_assoc.
+        - ss. }
+      unfold link in *. ss. desf.
+    - clear P1_2S.
+      exploit P12_3S.
+      { rewrite prog_defmap_elements.
+        rewrite PTree.gcombine by ss.
+        rewrite DEF1. rewrite DEF2. ss.
+      }
+      clear P12_3S. intro C12_3S.
+      destruct ((prog_defmap m3) ! x) as [d3| ] eqn: DEF3.
+      2: { unfold link_prog_check in *. desf. }
+
+      unfold link_prog_check in *. desf.
+      2: { clear -C12_3S. des_bool. ss. }
+
+      des_bool. des; ss.
+      des_bool. des.
+      + assert (IN1: In x (AST.prog_public m1)).
+        { unfold proj_sumbool in *.
+          desf.
+          rewrite in_app in *. des; ss.
+        }
+        inv WF1.
+        exploit PUBINCL; eauto.
+        i. exploit prog_defmap_dom; eauto. i. des.
+        congruence.
+      + congruence.
+  }
+
+  (* link 2_3 succ *)
+  destruct (link m1 m2) as [m12|] eqn: L1_2S.
+  2: { (* link 1_2 fail *)
+    ss. unfold link_prog in L2_3. unfold link_prog in L1_2S.
+    desf.
+    renames Heq0 Heq into C2_3S C1_2F.
+    des_bool. rename C2_3S1 into P2_3S. des.
+    { unfold link_prog. ss. desf. }
+
+    rewrite PTree_Properties.for_all_false in C1_2F.
+    destruct C1_2F as [x [d1 [DEF1 L1_2F]]].
+
+    rewrite PTree_Properties.for_all_correct in P2_3S. specialize (P2_3S x).
+    unfold link_prog_check in L1_2F.
+    destruct ((prog_defmap m2) ! x) as [d2| ] eqn: DEF2; ss.
+    exploit P2_3S; eauto.
+    clear P2_3S. intro C2_3S.
+
+    des_bool. des.
+    { des_bool. des.
+      - unfold link_prog. ss. desf. exfalso.
+        rename Heq into P1_23S. des_bool.
+        rename P1_23S1 into P1_23S.
+        rewrite PTree_Properties.for_all_correct in P1_23S.
+        exploit P1_23S; eauto. clear P1_23S. intro C1_23S.
+        unfold link_prog_check in C1_23S. desf.
+        clear C1_23S. rename Heq into C1_23S.
+
+        rewrite prog_defmap_elements in C1_23S.
+        rewrite PTree.gcombine in C1_23S by ss.
+
+        clear - DEF2 C2_3S C1_23S.
+        unfold link_prog_check, link_prog_merge in *. desf.
+        des_bool. ss.
+
+      - unfold link_prog. ss. desf. exfalso.
+        rename Heq into P1_23S. des_bool.
+        rename P1_23S1 into P1_23S.
+        rewrite PTree_Properties.for_all_correct in P1_23S.
+        exploit P1_23S; eauto. clear P1_23S. intro C1_23S.
+
+        unfold link_prog_check in C2_3S. ss.
+        destruct ((prog_defmap m3) ! x) as [d3|] eqn: DEF3.
+        { desf. }
+
+        assert (NOT_IN3: ~ In x (AST.prog_public m3)).
+        { ii. inv WF3.
+          exploit PUBINCL; eauto. i.
+          exploit prog_defmap_dom; eauto. i. des. congruence.
+        }
+
+        unfold link_prog_check in C1_23S.
+        rewrite prog_defmap_elements in C1_23S. ss.
+        rewrite PTree.gcombine in C1_23S by ss.
+        rewrite DEF2 in C1_23S. rewrite DEF3 in C1_23S. ss.
+
+        des_bool.
+        clear - L1_2F C1_23S3 NOT_IN3.
+        des_sumbool. rewrite in_app in *. des; ss.
+    }
+
+    desf. clear L1_2F. rename Heq into L1_2F.
+
+    unfold link_prog. ss. desf. exfalso.
+    rename Heq into P1_23S. des_bool.
+    rename P1_23S1 into P1_23S.
+
+    rewrite PTree_Properties.for_all_correct in P1_23S.
+    exploit P1_23S; eauto. clear P1_23S. intro C1_23S.
+
+    destruct ((prog_defmap m3)! x) as [d3|] eqn: DEF3.
+    - assert (exists d23, link_def d2 d3 = Some d23).
+      { clear C1_23S.
+        unfold link_prog_check in *.
+        rewrite DEF3 in *.
+        des_bool. ss. desf. esplits; eauto.
+      }
+      des.
+
+      assert (exists d123, link_def d1 d23 = Some d123).
+      { clear C2_3S.
+        unfold link_prog_check in *.
+        rewrite prog_defmap_elements in C1_23S.
+        rewrite PTree.gcombine in * by ss.
+        rewrite DEF2 in *. rewrite DEF3 in *. ss.
+        desf.
+        { esplits; eauto. }
+
+        exfalso.
+        des_bool. ss.
+      }
+      des.
+
+      assert (match link_def d1 d2 with
+              | Some d12 => link_def d12 d3
+              | None => None
+              end =
+              match link_def d2 d3 with
+              | Some d23 => link_def d1 d23
+              | None => None
+              end).
+      { apply link_def_assoc.
+        - apply link_skfundef_assoc.
+        - ss.
+      }
+      desf. congruence.
+    - unfold link_prog_check in C1_23S.
+      rewrite prog_defmap_elements in C1_23S. ss.
+      rewrite PTree.gcombine in C1_23S by ss.
+      rewrite DEF2 in C1_23S. rewrite DEF3 in C1_23S. ss.
+      des_bool. desf.
+  }
+
+  (* all succ *)
+
+  unfold link in *. ss.
+
+  destruct (link_prog m12 m3) as [[? ? ?]|] eqn: L12_3.
+  2: {
+    unfold link_prog in *.
+
+    des_matchH L1_2S L1_2_COND; ss.
+    des_matchH L12_3 L12_3_COND; ss.
+    des_matchH L2_3 L2_3_COND; ss.
+    clarify. des_bool.
+
+    des.
+    - exfalso. des_sumbool. ss. congruence.
+    - rewrite PTree_Properties.for_all_correct in *.
+      rewrite PTree_Properties.for_all_false in *. des.
+      destruct ((prog_defmap m1) ! x) as [gd1|] eqn: DEF1.
+      + exploit L1_2_COND1; eauto.
+        unfold link_prog_check.
+        destruct ((prog_defmap m2) ! x) as [gd2|] eqn: DEF2.
+        2: {
+          i. rewrite prog_defmap_elements in L12_3_COND.
+          rewrite PTree.gcombine in * by ss.
+          rewrite DEF1 in *. rewrite DEF2 in *. ss.
+          symmetry in L12_3_COND. clarify.
+          unfold link_prog_check in L12_3_COND0. ss.
+
+          destruct ((prog_defmap m3) ! x) as [gd3|] eqn: DEF3; ss.
+          desf.
+          - exfalso.
+            rename Heq into P1_23.
+            rewrite PTree_Properties.for_all_correct in *.
+            exploit P1_23; eauto. clear P1_23.
+            rewrite prog_defmap_elements.
+            rewrite PTree.gcombine by ss.
+            rewrite DEF2. ss.
+            des_bool. des; ss. des_bool.
+            rewrite DEF3.
+            do 2 rewrite andb_true_iff. i. desf.
+            + des_sumbool.
+              apply L12_3_COND0. apply in_app. eauto.
+            + des_sumbool.
+              rewrite in_app in *. des; ss.
+              inv WF2. exploit PUBINCL; eauto.
+              i. exploit prog_defmap_dom; eauto. i. des. congruence.
+
+          - exfalso.
+            rename Heq into P1_23.
+            rewrite PTree_Properties.for_all_correct in *.
+            exploit P1_23; eauto. clear P1_23.
+            rewrite prog_defmap_elements.
+            rewrite PTree.gcombine by ss.
+            rewrite DEF2. rewrite DEF3. ss.
+            do 2 rewrite andb_true_iff. i. des. desf.
+        }
+
+        i. des_bool.
+        destruct (link gd1 gd2) as [gd12| ] eqn: L1_2; ss.
+
+        rewrite prog_defmap_elements in L12_3_COND.
+        rewrite PTree.gcombine in * by ss.
+        rewrite DEF1 in *. rewrite DEF2 in *. ss.
+        move L1_2 at top. clarify.
+        unfold link_prog_check in L12_3_COND0. ss.
+
+        destruct ((prog_defmap m3) ! x) as [gd3|] eqn: DEF3; ss.
+        des_bool. des.
+        { exfalso.
+          des_bool. des.
+          - des_sumbool.
+            apply L12_3_COND0. apply in_app.
+            des; eauto.
+          - des_sumbool.
+            exploit L2_3_COND1; eauto.
+            unfold link_prog_check. rewrite DEF3.
+            i. des_bool. des_sumbool. congruence.
+        }
+
+        desf.
+        exfalso.
+        rename Heq into P1_23.
+        rewrite PTree_Properties.for_all_correct in *.
+        exploit P1_23; eauto. clear P1_23.
+        rewrite prog_defmap_elements.
+        rewrite PTree.gcombine by ss.
+        rewrite DEF2. rewrite DEF3. ss.
+
+        exploit L2_3_COND1; eauto.
+        unfold link_prog_check. rewrite DEF3.
+        i. ss. des_bool.
+        destruct (link_def gd2 gd3) as [gd23|] eqn: L2_3; ss.
+        des_bool.
+        destruct (link_def gd1 gd23) as [gd123|] eqn: L1_23; ss.
+
+        generalize (link_skdef_assoc gd1 gd2 gd3).
+        ss. rewrite L2_3. rewrite L1_23.
+        rewrite L12_3_COND. congruence.
+      +
+        exfalso.
+        rewrite prog_defmap_elements in L12_3_COND.
+        rewrite PTree.gcombine in L12_3_COND by ss.
+        rewrite DEF1 in *.
+
+        destruct ((prog_defmap m2) ! x) as [gd2|] eqn: DEF2; ss.
+        symmetry in L12_3_COND. clarify.
+
+        unfold link_prog_check in L12_3_COND0. ss.
+
+        destruct ((prog_defmap m3) ! x) as [gd3|] eqn: DEF3; ss.
+
+        exploit L2_3_COND1; eauto.
+        unfold link_prog_check. rewrite DEF3.
+        i. ss. des_bool.
+        destruct (link_def gd2 gd3) as [gd23|] eqn: L2_3; ss.
+        des; ss.
+        des_bool. des.
+        * des_sumbool. apply L12_3_COND0.
+          apply in_app. eauto.
+        * des_sumbool. ss.
+  }
+
+  rename L12_3 into L12_3S.
+  eapply link_prog_inv in L12_3S. des.
+  clarify.
+
+  unfold link_prog in L2_3.
+  des_matchH L2_3 L2_3S_COND; ss. des_bool. clarify.
+  unfold link_prog in L1_2S.
+  des_matchH L1_2S L1_2S_COND; ss. des_bool. clarify. ss.
+  rewrite PTree_Properties.for_all_correct in *.
+  des_sumbool.
+
+  rewrite link_prog_succeeds; ss.
+  - rewrite <- app_assoc.
+    f_equal. f_equal.
+    apply PTree.elements_extensional.
+    intro id.
+    do 2 rewrite PTree.gcombine by ss.
+
+    destruct ((prog_defmap m1) ! id) as [gd1|] eqn: DEF1;
+      destruct ((prog_defmap m2) ! id) as [gd2|] eqn: DEF2.
+    + exploit L1_2S_COND1; eauto.
+      unfold link_prog_check. rewrite DEF2.
+      do 2 rewrite andb_true_iff. intros [[? ?] L1_2S].
+      des_sumbool.
+      destruct (link gd1 gd2) as [gd12| ] eqn: LINK1_2; ss.
+
+      do 2 rewrite prog_defmap_elements.
+      do 2 rewrite PTree.gcombine by ss.
+      rewrite DEF1. rewrite DEF2. ss. rewrite LINK1_2. ss.
+
+      destruct ((prog_defmap m3) ! id) as [gd3|] eqn: DEF3; ss.
+      exploit L2_3S_COND1; eauto.
+      unfold link_prog_check. rewrite DEF3.
+      do 2 rewrite andb_true_iff. intros [[? ?] L2_3S].
+      des_sumbool.
+      destruct (link gd2 gd3) as [gd23| ] eqn: LINK2_3; ss.
+      rewrite LINK2_3.
+      generalize (link_skdef_assoc gd1 gd2 gd3). ss. desf.
+    + ss. do 2 rewrite prog_defmap_elements.
+      do 2 rewrite PTree.gcombine by ss.
+      rewrite DEF1. rewrite DEF2. ss.
+    + ss. do 2 rewrite prog_defmap_elements.
+      do 2 rewrite PTree.gcombine by ss.
+      rewrite DEF1. rewrite DEF2. ss.
+    + ss. do 2 rewrite prog_defmap_elements.
+      do 2 rewrite PTree.gcombine by ss.
+      rewrite DEF1. rewrite DEF2. ss.
+  - setoid_rewrite prog_defmap_elements.
+    setoid_rewrite PTree.gcombine.
+    2: { ss. }
+    intros x gd1 gd23 DEF1 DEF23.
+    exploit L1_2S_COND1; eauto. unfold link_prog_check.
+
+    destruct ((prog_defmap m2) ! x) as [gd2|] eqn: DEF2.
+    2: { i. exploit L12_3S0; eauto.
+         { rewrite prog_defmap_elements.
+           rewrite PTree.gcombine by ss.
+           rewrite DEF1. rewrite DEF2. ss.
+         }
+
+         i. des.
+         rewrite in_app in *. des.
+         - splits; auto. congruence.
+         - exfalso. inv WF2.
+           exploit PUBINCL; eauto. i.
+           exploit prog_defmap_dom; eauto. i. des. congruence.
+    }
+
+    do 2 rewrite andb_true_iff.
+
+    destruct (link gd1 gd2) as [gd12|] eqn: L1_2.
+    2: { i. des. ss. }
+    i. des.
+    des_sumbool.
+    splits; auto.
+    { apply in_app; auto. }
+
+    destruct ((prog_defmap m3) ! x) as [gd3| ] eqn: DEF3; ss.
+    2: { clarify. congruence. }
+    generalize (link_skdef_assoc gd1 gd2 gd3). ss. desf.
+    intro R. rewrite <- R.
+    exploit L12_3S0; eauto.
+    { rewrite prog_defmap_elements.
+      rewrite PTree.gcombine by ss.
+      rewrite DEF1. rewrite DEF2. eauto. }
+
+    i. des. congruence.
+Qed.
+
+
+
+
+
+Theorem link_list_prepend_eq
+      (sk0 sk1 sk2: list Sk.t)
+      (NOEMPTY: sk0 <> [] /\ sk1 <> [])
+      (SAME: link_list sk0 = link_list sk1):
+    <<EQ: link_list (sk2 ++ sk0) = link_list (sk2 ++ sk1)>>.
+Proof.
+  r. ginduction sk2; ss.
+  ii. unfold link_sk in *. ss.
+  exploit IHsk2; eauto. i.
+  clear - NOEMPTY H. unfold link_list in H. des_ifs; ss.
+  - unfold link_list. ss. rewrite Heq. rewrite Heq0. ss.
+  - des. eapply link_list_aux_empty_inv in Heq. destruct sk2; destruct sk0; ss.
+  - des. eapply link_list_aux_empty_inv in Heq0. destruct sk2; destruct sk1; ss.
+  - unfold link_list. ss. rewrite Heq, Heq0. auto.
+  - unfold link_list. ss. rewrite Heq, Heq0. auto.
+Qed.
+
+Theorem link_list_assoc_one
+      (ctx: list Sk.t) sk0 sk1 sk_link
+      (WF0: Sk.wf sk0)
+      (WF1: Sk.wf sk1)
+      (WFLINK: Sk.wf sk_link)
+      (LINK: link sk0 sk1 = Some sk_link)
+      (WFCTX: forall sk, In sk ctx -> Sk.wf sk)
+  :
+    <<EQ: link_list ([sk0 ; sk1] ++ ctx) = link_list ([sk_link] ++ ctx)>>
+.
+Proof.
+  unfold link_list.
+  remember (link_list_aux ctx) as link_ctx.
+  destruct link_ctx; ss.
+  { des_ifs. }
+  { des_ifs. }
+
+  exploit (@link_sk_assoc sk0 sk1 t); eauto.
+  { eapply link_list_preserves_wf_sk; et. unfold link_list. des_ifs. }
+  intro R.
+  ss. desf; congruence.
+Qed.
+
+Theorem link_list_assoc
+        (sk0 sk1 sk2: list Sk.t)
+  :
+    <<EQ: link_list (sk0 ++ sk1 ++ sk2) = link_list ((sk0 ++ sk1) ++ sk2)>>
+.
+Proof.
+  ginduction sk0; ii; ss.
+  destruct (classic (sk0 ++ sk1 ++ sk2 = nil)).
+  { destruct sk0, sk1, sk2; ss. }
+  replace (a :: sk0 ++ sk1 ++ sk2) with ([a] ++ (sk0 ++ sk1 ++ sk2)) by ss.
+  replace (a :: (sk0 ++ sk1) ++ sk2) with ([a] ++ ((sk0 ++ sk1) ++ sk2)) by ss.
+  eapply link_list_prepend_eq with (sk2 := [a]); ss.
+  { destruct sk0, sk1, sk2; ss. }
+  rewrite IHsk0; et.
+Qed.
+
+Lemma link_sk_prepend_eq
+      A B C
+      (NOEMPTY: A <> [] /\ B <> [])
+      (SAME: link_sk A = link_sk B):
+    link_sk (C ++ A) = link_sk (C ++ B).
+Proof.
+  unfold link_sk in *. rewrite ! map_app. eapply link_list_prepend_eq; et.
+  des. destruct A, B; ss.
+Qed.
+
+Lemma link_sk_assoc_one ctx (mA mB mL: Mod.t)
+      (WFA: Sk.wf mA)
+      (WFB: Sk.wf mB)
+      (WFL: Sk.wf mL)
+      (LINK_OK: link (Mod.sk mA) (Mod.sk mB) = Some (Mod.sk mL))
+      (WFCTX: forall md : Mod.t, In md ctx -> Sk.wf md)
+  : link_sk ([mA; mB] ++ ctx)
+    = link_sk ([mL] ++ ctx).
+Proof.
+  unfold link_sk. ss.
+  apply link_list_assoc_one; ss. ii. rewrite in_map_iff in *. des; clarify. et.
+Qed.
+
+Lemma link_sk_main_eq
+      ms sk
+      (LINK_OK: link_sk ms = Some sk)
+  : List.Forall (fun m => AST.prog_main (Mod.sk m) = AST.prog_main sk) ms.
+Proof.
+  Local Transparent Linker_prog.
+  depgen sk.
+  induction ms as [|ms]; i; ss.
+  unfold link_sk in *. ss.
+  unfold link_list in *. ss. desf.
+  - destruct ms0; ss.
+    2: { desf. }
+    econs; ss.
+  - exploit IHms; eauto. i.
+    match goal with
+    | H: link_prog _ _ = Some _ |- _ =>
+      eapply link_prog_inv in H
+    end.
+    des. clarify. ss.
+    econs; eauto.
+    replace (AST.prog_main (Mod.sk ms)) with (AST.prog_main t). ss.
+    Local Opaque Linker_prog.
+Qed.
+
+
+Lemma linkorder_internal_max
+      fsig (gd: globdef (AST.fundef signature) unit)
+      (LO: linkorder (Gfun (AST.Internal fsig)) gd)
+  : gd = (Gfun (AST.Internal fsig)).
+Proof.
+  Local Transparent Linker_def.
+  ss. inv LO.
+  match goal with
+  | H : linkorder _ _ |- _ => inv H
+  end. reflexivity.
+  Local Opaque Linker_def.
+Qed.
+
+Lemma globdef_linkorder
+      skT gdT gid
+      (skA skB skL: Sk.t)
+      (sk_link_ok: link skA skB = Some skL)
+      (FOCUS: skT = skA \/ skT = skB)
+      (DEF_T: (prog_defmap skT) ! gid = Some gdT)
+  : exists gdL, <<DEF_L: (prog_defmap skL) ! gid = Some gdL>> /\
+                    <<LO: linkorder gdT gdL>>.
+Proof.
+  exploit (link_prog_inv skA skB skL).
+  { apply sk_link_ok. }
+  intros [MAIN_EQ [DEFMAP_LINK SKL]].
+
+  des; clarify.
+  - destruct ((prog_defmap skB) ! gid) as [gdB|] eqn: DEF_O.
+    + exploit DEFMAP_LINK; eauto.
+      intros [IN_SKA [IN_SKB [gdL LINK_SOME]]].
+      (* rewrite SKL. *)
+      rewrite prog_defmap_elements.
+      rewrite PTree.gcombine by ss.
+      rewrite DEF_T. rewrite DEF_O. ss.
+      esplits; eauto.
+      eapply link_linkorder in LINK_SOME.
+      des. eauto.
+    + (* rewrite SKL. *)
+      rewrite prog_defmap_elements.
+      rewrite PTree.gcombine by ss.
+      rewrite DEF_T. rewrite DEF_O. ss.
+      esplits; eauto.
+      apply linkorder_refl.
+  - destruct ((prog_defmap skA) ! gid) as [gdA|] eqn: DEF_O.
+    + exploit DEFMAP_LINK; eauto.
+      intros [IN_SKA [IN_SKB [gdL LINK_SOME]]].
+      (* rewrite SKL. *)
+      rewrite prog_defmap_elements.
+      rewrite PTree.gcombine by ss.
+      rewrite DEF_T. rewrite DEF_O. ss.
+      esplits; eauto.
+      eapply link_linkorder in LINK_SOME.
+      des. eauto.
+    + (* rewrite SKL. *)
+      rewrite prog_defmap_elements.
+      rewrite PTree.gcombine by ss.
+      rewrite DEF_T. rewrite DEF_O. ss.
+      esplits; eauto.
+      apply linkorder_refl.
+Qed.
+
+Lemma prog_defmap_internal_impl
+      skenv sk fid fsig
+      (DEF_INT: (prog_defmap sk)!fid = Some (Gfun (AST.Internal fsig)))
+      (INCL: SkEnv.includes skenv sk)
+  : exists blk,
+    (<<SKENV_SYMBOL: Genv.find_symbol skenv fid = Some blk>> /\
+     <<SKENV_FUNCT_PTR: Genv.find_funct_ptr skenv blk = Some (AST.Internal fsig)>>) /\
+    (<<PROJ_SYMBOL: Genv.find_symbol (SkEnv.project skenv sk) fid = Some blk>> /\
+     <<PROJ_FUNCT_PTR: Genv.find_funct_ptr (SkEnv.project skenv sk) blk = Some (AST.Internal fsig)>>).
+Proof.
+  pose proof INCL as INCL2.
+  inv INCL2. exploit DEFS; eauto. i. des.
+  exploit linkorder_internal_max; eauto.
+  i. subst.
+
+  exists blk.
+  pose proof DEF as DEF2.
+  apply Genv.find_funct_ptr_iff in DEF2.
+  split.
+  { split; auto. }
+
+  assert (internals sk fid = true) by (unfold internals; desf).
+  hexploit (SkEnv.project_impl_spec INCL); eauto. intro PROJ. inv PROJ.
+  rewrite SYMBKEEP by (apply internals_defs; eauto).
+  split; auto.
+
+  apply Genv.find_funct_ptr_iff.
+  exploit DEFKEEP; eauto.
+  { apply Genv.find_invert_symbol. auto. }
+  i. des. rewrite DEFSMALL. congruence.
+Qed.
+
+
+Lemma link_defs
+      (sk1 sk2 skl: Sk.t) fid
+      (LINK: link sk1 sk2 = Some skl)
+      (DEF_TGT: defs sk1 fid \/ defs sk2 fid)
+  : defs skl fid.
+Proof.
+  unfold defs in *. des; des_sumbool.
+  - rewrite prog_defmap_spec in *. des.
+    exploit globdef_linkorder; try apply LINK; try apply DEF_TGT; eauto.
+    i. des. eauto.
+  - rewrite prog_defmap_spec in *. des.
+    exploit globdef_linkorder; try apply LINK; try apply DEF_TGT; eauto.
+    i. des. eauto.
+Qed.
+
+Section MORE_LINK_LEMMAS.
+  Variable ms: list Mod.t.
+  Variable sk_link : Sk.t.
+  Hypothesis SK_LINK: link_sk ms = Some sk_link.
+  Let skenv := Sk.load_skenv sk_link.
+  Hypothesis MODS_WF: forall md : Mod.t, In md ms -> Sk.wf md.
+
+  Lemma ge_disjoint
+    : Ge.disjoint (load_genv ms skenv).
+  Proof.
+    cut (Ge.disjoint (Smallstep.globalenv (sem ms))).
+    { ss. rewrite SK_LINK. eauto. }
+
+    apply SemProps.genv_disjoint.
+  Qed.
+
+  Section INCL.
+    Variable sk: Sk.t.
+    Variable m: Mod.t.
+    Hypothesis MOD_SK: Mod.sk m = sk.
+    Hypothesis MOD_IN_MS: In m ms.
+
+    (* Let m : Mod.t := ITreeMod.to_mod sk im. *)
+
+    Lemma incl_sk: SkEnv.includes skenv sk.
+    Proof.
+      unfold skenv.
+      exploit link_includes; eauto. clarify.
+    Qed.
+  End INCL.
+End MORE_LINK_LEMMAS.
